enable sot_wds,rotate*,is_balanced

test.c
@@ -5,6 +5,7 @@ int main() {
   printf("r=%ui\n", p);
   uint64_t h = P1_UInt32_main2 ();
   printf("h=%ui\n", h);
-  printf("Hello, world!\n");
+  uint64_t s = P1_UInt32_main3 ();
+  printf("s=%ui\n", s);
   return 0;
 }
